Code reorganization around Spec.Hash.Incremental

specs/Spec.Hash.Lemmas.fst
@@ -6,7 +6,6 @@ include Spec.Hash.Lemmas0
 
 open Spec.Agile.Hash
 open Spec.Hash.Definitions
-open Spec.Hash.Incremental
 open Spec.Hash.PadFinish
 
 friend Spec.Agile.Hash
@@ -33,74 +32,3 @@ let update_multi_associative (a: hash_alg)
       (update_multi a h input)))
 =
   Lib.UpdateMulti.update_multi_associative (block_length a) (Spec.Agile.Hash.update a) h input1 input2
-
-#set-options "--max_fuel 0 --max_ifuel 0 --z3rlimit 50"
-
-let blake2_is_hash_incremental
-  (a:hash_alg{is_blake a}) (d:bytes{Seq.length d <= max_input_length a})
-  : Lemma
-    (Spec.Blake2.blake2 (to_blake_alg a) d 0 Seq.empty (Spec.Blake2.max_output (to_blake_alg a)) ==
-     Spec.Hash.Incremental.hash_incremental a d)
-  = admit()
-
-let hash_is_hash_incremental (a: hash_alg) (input: bytes { S.length input <= max_input_length a }):
-  Lemma (ensures (S.equal (hash a input) (hash_incremental a input)))
-=
-  if is_blake a then blake2_is_hash_incremental a input
-  else
-  admit();
-  let open FStar.Mul in
-  let n = S.length input / block_length a in
-  let padding = pad a (S.length input) in
-  let padded_input = input `S.append` padding in
-  let blocks, rest = Lib.UpdateMulti.split_block (block_length a) padded_input n in
-  let blocks', rest' = S.split input (n * block_length a) in
-  S.lemma_eq_intro blocks blocks';
-  S.lemma_eq_intro (rest' `S.append` padding) rest;
-  Math.Lemmas.multiple_modulo_lemma n (block_length a);
-  S.lemma_eq_intro padded_input (blocks `S.append` rest);
-  update_multi_associative a (init a) blocks rest;
-  S.lemma_eq_intro (fst (update_multi a (init a) padded_input)) (fst (update_multi a (update_multi a (init a) blocks) rest))
-
-#push-options "--z3rlimit 100"
-
-let concatenated_hash_incremental_md (a:hash_alg{is_md a}) (inp1:bytes_blocks a) (inp2:bytes)
-  : Lemma
-    (requires Seq.length (inp1 `S.append` inp2) <= max_input_length a)
-    (ensures finish a (update_last a (update_multi a (init a) inp1) (S.length inp1) inp2)
-      `S.equal` Spec.Hash.Incremental.hash_incremental a (inp1 `S.append` inp2))
-  = admit();
-    allow_inversion hash_alg;
-    let len = S.length inp2 in
-    calc (S.equal) {
-    finish a (update_last a (update_multi a (init a) inp1)
-        (S.length inp1) inp2);
-    (S.equal) { }
-      finish a (update_multi a (update_multi a (init a) inp1)
-        (S.append inp2 (pad a (S.length inp1 + len))));
-    (S.equal) { }
-      finish a (update_multi a (init a)
-        (S.append inp1
-          (S.append inp2 (pad a (S.length inp1 + len)))));
-    (S.equal) { S.append_assoc
-      inp1
-      inp2
-      (pad a (S.length inp1 + len))
-    }
-      finish a (update_multi a (init a)
-        (S.append (S.append inp1 inp2)
-          (pad a (S.length inp1 + len))));
-    (==) { }
-      Spec.Agile.Hash.hash a (S.append inp1 inp2);
-    };
-    hash_is_hash_incremental a (S.append inp1 inp2)
-
-#pop-options
-
-let concatenated_hash_incremental (a:hash_alg) (inp1:bytes_blocks a) (inp2:bytes)
-  : Lemma
-    (requires Seq.length (inp1 `S.append` inp2) <= max_input_length a)
-    (ensures finish a (update_last a (update_multi a (init a) inp1) (S.length inp1) inp2)
-      `S.equal` Spec.Hash.Incremental.hash_incremental a (inp1 `S.append` inp2))
-   = if is_blake a then admit() // proven in Spec.Hash.Incremental, todo, reorganize
-     else concatenated_hash_incremental_md a inp1 inp2
