specs/Spec.Hash.Lemmas.fsti
@@ -6,7 +6,6 @@ include Spec.Hash.Lemmas0
 
 open Spec.Agile.Hash
 open Spec.Hash.Definitions
-open Spec.Hash.Incremental
 open Spec.Hash.PadFinish
 
 val update_multi_zero (a: hash_alg) (h: words_state a): Lemma
@@ -29,14 +28,3 @@ val update_multi_associative (a: hash_alg)
     (update_multi a (update_multi a h input1) input2) ==
       (update_multi a h input)))
   [ SMTPat (update_multi a (update_multi a h input1) input2) ]
-
-let hash = Spec.Agile.Hash.hash
-
-val hash_is_hash_incremental (a: hash_alg) (input: bytes { S.length input <= max_input_length a }):
-  Lemma (ensures (S.equal (hash a input) (hash_incremental a input)))
-
-val concatenated_hash_incremental (a:hash_alg) (inp1:bytes_blocks a) (inp2:bytes)
-  : Lemma
-    (requires Seq.length (inp1 `S.append` inp2) <= max_input_length a)
-    (ensures finish a (update_last a (update_multi a (init a) inp1) (S.length inp1) inp2)
-      `S.equal` hash_incremental a (inp1 `S.append` inp2))
