specs/lemmas/Spec.Hash.Incremental.Lemmas.fsti
@@ -1,0 +1,11 @@
+module Spec.Hash.Incremental.Lemmas
+
+module S = FStar.Seq
+
+open Spec.Hash.Definitions
+open Spec.Hash.Incremental
+
+let hash = Spec.Agile.Hash.hash
+
+val hash_is_hash_incremental (a: hash_alg) (input: bytes { S.length input <= max_input_length a }):
+  Lemma (ensures (S.equal (hash a input) (hash_incremental a input)))
