specs/lemmas/Spec.Hash.Incremental.fsti
@@ -1,0 +1,56 @@
+module Spec.Hash.Incremental
+
+module S = FStar.Seq
+
+open Spec.Agile.Hash
+open Spec.Hash.Definitions
+open Spec.Hash.PadFinish
+open FStar.Mul
+open Lib.IntTypes
+
+#set-options "--max_fuel 0 --max_ifuel 0 --z3rlimit 300"
+
+let update_last_blake (a:hash_alg{is_blake a})
+  (hash:words_state a)
+  (prevlen:nat{prevlen % block_length a = 0})
+  (input:bytes{S.length input + prevlen <= max_input_length a}):
+  Tot (words_state a)
+  = let (nb, rem) = Spec.Blake2.split (to_blake_alg a) (S.length input) in
+    let blocks = Seq.slice input 0 (nb * block_length a) in
+    let (h', totlen) = update_multi a hash blocks in
+    let last_block = Spec.Blake2.get_last_padded_block (to_blake_alg a) input rem in
+    (Spec.Blake2.blake2_update_block (to_blake_alg a) true (v (totlen +. u64 rem)) last_block h', u64 0)
+
+(* An incremental specification better suited to a stateful API, allowing the
+   client to perform the padding at the last minute upon hitting the last chunk of
+   data. *)
+let update_last (a:hash_alg)
+  (hash:words_state a)
+  (prevlen:nat{prevlen % block_length a = 0})
+  (input:bytes{S.length input + prevlen <= max_input_length a}):
+  Tot (words_state a)
+=
+  if is_blake a then
+    update_last_blake a hash prevlen input
+  else
+  let total_len = prevlen + S.length input in
+  let padding = pad a total_len in
+  update_multi a hash S.(input @| padding)
+
+let hash_incremental (a:hash_alg) (input:bytes{S.length input <= (max_input_length a)}):
+  Tot (hash:bytes{S.length hash = (hash_length a)})
+=
+  let open FStar.Mul in
+  let n = S.length input / (block_length a) in
+  // Ensuring that we always handle one block in update_last
+  let n = if S.length input % block_length a = 0 && n > 0 then n-1 else n in
+  let bs, l = S.split input (n * (block_length a)) in
+  let hash = update_multi a (init a) bs in
+  let hash = update_last a hash (n * (block_length a)) l in
+  finish a hash
+
+val concatenated_hash_incremental (a:hash_alg) (inp1:bytes_blocks a) (inp2:bytes)
+  : Lemma
+    (requires Seq.length (inp1 `S.append` inp2) <= max_input_length a /\ Seq.length inp2 > 0)
+    (ensures finish a (update_last a (update_multi a (init a) inp1) (S.length inp1) inp2)
+      `S.equal` hash_incremental a (inp1 `S.append` inp2))
